bin/rust/rocq/SymexSoundness.v
@@ -1,0 +1,166 @@
+From iris.proofmode Require Import proofmode.
+Require Export AxSem LogicalHeaps.
+
+Instance EqDecision_Ty: EqDecision Ty.
+Admitted.
+
+Instance Countable_Ty: Countable Ty.
+Admitted.
+
+Instance EqDecision_Ptr: EqDecision Ptr.
+Admitted.
+
+Instance Countable_Ptr: Countable Ptr.
+Admitted.
+
+Definition PhysHeap := gmap (Ty * Ptr) Value.
+
+Definition logheap_of_physheap(hp: PhysHeap): LogHeap :=
+  map_fold (fun '(ty, ptr) v H => {[+ PointsTo_ ty (VPtr ptr) v +]} ⋅ H) ∅ hp.
+
+Section gfunctors.
+
+Context {Σ: gFunctors}.
+
+Definition own_physheap(hp: PhysHeap): iProp Σ :=
+  [∗ map] '(ty, ptr) ↦ v ∈ hp, points_to_ ty (VPtr ptr) v.
+
+Definition place_as_ptr(env: AxSem.Env)(place: Place): Value :=
+  match place with
+    PNonAddrTakenLocal x => VPtr (snd (env x))
+  | PDeref ptr => ptr
+  end.
+
+Section preds.
+
+Variable preds: list (string * PredDef).
+
+Definition own_heap(h: Heap): iProp Σ :=
+  ∃ hp,
+  ⌜ heap_holds preds (logheap_of_physheap hp) h ⌝ ∗
+  own_physheap hp.
+
+Definition own_env_entry(Γ: AxSem.Env)(x: string)(state: LocalState): iProp Σ :=
+  match state with
+    LSValue v => points_to (fst (Γ x)) (VPtr (snd (Γ x))) v
+  | LSPlace ptr => ⌜ ptr = snd (Γ x) ⌝
+  end.
+
+Fixpoint own_env(Γ: AxSem.Env)(env: Env): iProp Σ :=
+  match env with
+    [] => True
+  | (x, state)::env => own_env_entry Γ x state ∗ own_env Γ env
+  end.
+
+Inductive place_has_ty(Γ: AxSem.Env): Place -> Ty -> Prop :=
+| PNonAddrTakenLocal_has_ty x:
+  place_has_ty Γ (PNonAddrTakenLocal x) (fst (Γ x))
+| PDeref_has_ty ptr ty:
+  place_has_ty Γ (PDeref ptr) ty
+.
+
+Lemma load_from_non_addr_taken_local Γ env x v:
+  assoc x env = Some (LSValue v) →
+  own_env Γ env -∗
+  points_to (Γ x).1 (VPtr (Γ x).2) v ∗
+  (points_to (Γ x).1 (VPtr (Γ x).2) v -∗ own_env Γ env).
+Proof.
+  induction env.
+  - (* nil *)
+    intros.
+    discriminate.
+  - (* cons *)
+    destruct a as [x' state].
+    intros.
+    simpl in *.
+    destruct (string_dec x x').
+    + subst.
+      injection H; clear H; intros; subst.
+      iStartProof.
+      iIntros "[H11 H12]".
+      iSplitL "H11".
+      * iExact "H11".
+      * iIntros "H2".
+        iSplitL "H2"; iAssumption.
+    + apply IHenv in H.
+      iStartProof.
+      iIntros "[H1 H2]".
+      iPoseProof (H with "H2") as "[H H']".
+      iSplitL "H".
+      iExact "H".
+      iIntros "H".
+      iSplitL "H1".
+      iAssumption.
+      iApply "H'".
+      iAssumption.
+Qed.
+
+Lemma consume_points_to_sound trace h tree ty ptr Qsymex Q:
+  consume_points_to trace h tree ty ptr Qsymex →
+  (∀ h tree v, Qsymex h tree v → own_heap h -∗ Q v) →
+  own_heap h -∗
+  ∃ v,
+  points_to ty ptr v ∗ Q v.
+Proof.
+  intros.
+  unfold own_heap.
+  iIntros "H".
+  iDestruct "H" as (hp) "[H1 H2]".
+  iDestruct "H1" as %H1.
+  apply consume_points_to_sound with (1:=H1) in H.
+  destruct H as (H' & h' & tree' & v & Hhp & Hh' & HQsymex).
+  apply H0 in HQsymex.
+  
+Qed.
+
+Lemma load_from_pointer_sound trace h tree ty ptr Qsymex Q:
+  load_from_pointer trace h tree ty ptr Qsymex →
+  (∀ h tree v, Qsymex h tree v → own_heap h -∗ Q v) →
+  own_heap h -∗
+  ∃ v,
+  points_to ty ptr v ∗
+  (points_to ty ptr v -∗ Q v).
+
+Lemma load_from_place_sound trace h env tree place ty Qsymex Γ Q:
+  load_from_place trace h env tree place ty Qsymex →
+  place_has_ty Γ place ty →
+  (∀ h tree v, Qsymex h tree v → own_heap h -∗ own_env Γ env -∗ Q v) →
+  own_heap h -∗
+  own_env Γ env -∗
+  ∃ v,
+  points_to ty (place_as_ptr Γ place) v ∗
+  (points_to ty (place_as_ptr Γ place) v -∗
+   Q v).
+Proof.
+  intros.
+  iStartProof.
+  iIntros "Hh Henv".
+  destruct place.
+  - (* PNonAddrTakenLocal *)
+    simpl in H.
+    simpl.
+    inversion H0; subst.
+    case_eq (assoc x env); intros; rewrite H2 in H; try tauto.
+    rename l into state.
+    destruct state; try tauto.
+    iExists v.
+    iPoseProof (load_from_non_addr_taken_local with "Henv") as "[H1 H2]".
+    apply H2.
+    iSplitL "H1". iAssumption.
+    iIntros "H".
+    iPoseProof ((H1 h tree v H) with "Hh") as "H'".
+    iApply "H'".
+    iApply "H2".
+    iAssumption.
+  - (* PDeref *)
+    simpl in H.
+
+Lemma verify_place_expr_elem_sound trace h env tree place ty place_expr_elem Qsymex Γ ptr Q:
+  verify_place_expr_elem trace h env tree place ty place_expr_elem Qsymex →
+  ptr = place_as_ptr Γ place →
+  (∀ h tree place ty, Qsymex h tree place ty → own_heap h -∗ own_env Γ env -∗ Q (place_as_ptr Γ place) ty) →
+  own_heap h -∗
+  own_env Γ env -∗
+  wp_PlaceExprElem ptr ty place_expr_elem Q.
+Proof.
+  
